tests/fuzzer/Fuzzer.ml
@@ -359,6 +359,8 @@ module Fuzzer (P: EngineParameters) (S: Warblre_js.Encoding.StringLike with type
             let name = M.find_opt (!group_id) names_map in
             group_id := (!group_id) + 1;
             Group (name, iter r1)
+        | ModifyGroupAdd (add, r1) -> ModifyGroupAdd (add, iter r1)
+        | ModifyGroupAddRemove (add, remove, r1) -> ModifyGroupAddRemove (add, remove, iter r1)
         | InputStart | InputEnd | WordBoundary | NotWordBoundary -> r
         | Lookahead (r1) -> Lookahead (iter r1)
         | NegativeLookahead (r1) -> NegativeLookahead (iter r1)
