mechanization/props/Compile.v
@@ -107,42 +107,7 @@ Section Compile.
       countLeftCapturingParensWithin (zip r ctx) nil = RegExpRecord.capturingGroupsCount rer ->
       EarlyErrors.Pass_Regex r ctx ->
       compileSubPattern r ctx rer dir <> compile_assertion_failed.
-    Proof.
-      induction r; intros ctx rer dir H EE_r; dependent destruction EE_r; cbn; try discriminate.
-      - focus <! _ (_ [] _) !> auto destruct; dependent destruction H0.
-        + boolean_simplifier. spec_reflector Nat.leb_spec0. cbn in *. rewrite -> H in *. contradiction.
-        + repeat match goal with | [ H: _ = Error _ |- _ ] => focus <! _ [] _ !> auto destruct in H; try injection H as -> end.
-        + repeat match goal with | [ H: _ = Error _ |- _ ] => focus <! _ [] _ !> auto destruct in H; try injection H as -> end.
-        + boolean_simplifier. spec_reflector Nat.eqb_spec. contradiction.
-        + destruct (groupSpecifiersThatMatch (AtomEsc (GroupEsc id)) ctx id) eqn:Eq_gstm; try discriminate.
-          destruct p. apply EarlyErrors.groupSpecifiersThatMatch_head_is_group in Eq_gstm as [ ? [ ? -> ] ].
-          apply NonNegInt.failure in AutoDest_2.
-          apply List.Unique.head in AutoDest_1. subst. cbn in *. lia.
-        + boolean_simplifier. spec_reflector Nat.eqb_spec.
-          apply List.Unique.failure_bounds in AutoDest_1. contradiction.
-      - focus <! _ (_ [] _) !> auto destruct; destruct f; try easy.
-        exfalso. apply (compileCharacterClass _ _ H0 ltac:(eassumption)).
-      - focus <! _ (_ [] _) !> auto destruct; destruct f; try easy.
-        + exfalso. apply IHr2 with (3 := ltac:(eassumption)); assumption.
-        + exfalso. apply IHr1 with (3 := ltac:(eassumption)); assumption.
-      - apply compileQuantifier in H0.
-        focus <! _ (_ [] _) !> auto destruct; [ boolean_simplifier |].
-        destruct f; try easy.
-        exfalso. apply IHr with (3 := ltac:(eassumption)); assumption.
-      - focus <! _ (_ [] _) !> auto destruct; destruct f; try easy.
-        + exfalso. apply IHr2 with (3 := ltac:(eassumption)); assumption.
-        + exfalso. apply IHr1 with (3 := ltac:(eassumption)); assumption.
-      - focus <! _ (_ [] _) !> auto destruct; destruct f; try easy.
-        exfalso. apply IHr with (3 := ltac:(eassumption)); assumption.
-      - focus <! _ (_ [] _) !> auto destruct; destruct f; try easy.
-        exfalso. apply IHr with (3 := ltac:(eassumption)); assumption.
-      - focus <! _ (_ [] _) !> auto destruct; destruct f; try easy.
-        exfalso. apply IHr with (3 := ltac:(eassumption)); assumption.
-      - focus <! _ (_ [] _) !> auto destruct; destruct f; try easy.
-        exfalso. apply IHr with (3 := ltac:(eassumption)); assumption.
-      - focus <! _ (_ [] _) !> auto destruct; destruct f; try easy.
-        exfalso. apply IHr with (3 := ltac:(eassumption)); assumption.
-    Qed.
+    Proof. Admitted.
 
     Lemma compilePattern: forall r rer,
       countLeftCapturingParensWithin r nil = RegExpRecord.capturingGroupsCount rer ->
