mechanization/spec/RegExpRecord.v
@@ -23,8 +23,7 @@ Module RegExpRecord.
     (*>> [[Unicode]] <<*)
     unicode: unit;
     (*>> [[UnicodeSets]] <<*)
-    (* + The UnicodeSets field is referenced in UpdateModifiers (22.2.2.7.4) but not currently represented in this record. +*)
-    (* + NEED: Add unicodeSets field to RegExpRecord for full compliance with RegExp Modifiers. +*)
+    unicodeSets: bool;
     (*>> [[CapturingGroupsCount]] <<*)
     capturingGroupsCount: non_neg_integer;
   }.
